Hooked up extern Array properly, implemented in C#

Source/DafnyRuntime/DafnyRuntimeDafny/test/externs.cs
@@ -1,0 +1,68 @@
+using System;
+using System.Numerics;
+
+namespace AtomicBoxes {
+
+  public class AtomicBox<T> where T : class {
+
+    private volatile T value;
+
+    public static AtomicBox<T> Make(T value) {
+      var result = new AtomicBox<T>();
+      result.Put(value);
+      return result;
+    }
+
+    public T Get() => value;
+    public void Put(T t) => value = t;
+  }
+}
+
+namespace Arrays {
+
+  public class __default {
+    public static Arrays.Array<T> NewArray<T>(BigInteger length) {
+      return new CsharpArray<T>((int)length);
+    }
+  }
+
+  public class CsharpArray<T> : Arrays.Array<T>, Arrays.ImmutableArray<T> {
+    private readonly T[] values;
+    private readonly int length;
+
+    public CsharpArray(int length) {
+      this.values = new T[length];
+      this.length = length;
+    }
+    
+    public CsharpArray(T[] values, int length) {
+      this.values = values;
+      this.length = length;
+    }
+
+    public BigInteger Length() {
+      return length;
+    }
+
+    public T Read(BigInteger i) {
+      return values[(int)i];
+    }
+    
+    public T At(BigInteger i) {
+      return values[(int)i];
+    }
+
+    public void Write(BigInteger i, T t) {
+      values[(int)i] = t;
+    }
+
+    public void WriteRangeArray(BigInteger start, Arrays.ImmutableArray<T> other) {
+      var csharpArray = other as CsharpArray<T>;
+      Array.Copy(csharpArray.values, 0, values, (int)start, csharpArray.length);
+    }
+
+    public Arrays.ImmutableArray<T> Freeze(BigInteger size) {
+      return new CsharpArray<T>(values, (int)size);
+    }
+  }
+}
