Source/DafnyRuntime/DafnyRuntimeDafny/src/array.dfy
@@ -4,7 +4,7 @@ include "../../../../Test/libraries/src/Math.dfy"
 
 include "frames.dfy"
 
-module {:extern} {:options "/functionSyntax:4"} Arrays {
+module {:extern "Arrays"} {:options "/functionSyntax:4"} Arrays {
 
   import opened Frames
   import opened Math
@@ -30,7 +30,9 @@ module {:extern} {:options "/functionSyntax:4"} Arrays {
   //    code amenable to such optimizations. :)
   //    See https://github.com/dafny-lang/dafny/issues/2447.
   //
-  trait {:extern} Array<T> extends Validatable {
+  // Has {:termination false} just so we can provide a feasibility implementation
+  // in a different file.
+  trait {:extern} {:termination false} Array<T> extends Validatable {
 
     ghost var values: seq<ArrayCell<T>>
 
@@ -54,18 +56,6 @@ module {:extern} {:options "/functionSyntax:4"} Arrays {
       ensures Repr == old(Repr)
       ensures values == old(values)[..i] + [Set(t)] + old(values)[(i + 1)..]
       ensures Read(i) == t
-
-    method WriteRange(start: nat, from: seq<T>)
-      requires Valid()
-      requires start <= Length()
-      requires start + |from| <= Length()
-      modifies Repr
-      ensures Valid()
-      ensures Repr == old(Repr)
-      ensures values == 
-        old(values)[..start] + 
-        seq(|from|, i requires 0 <= i < |from| => Set(from[i])) + 
-        old(values)[(start + |from|)..]
 
     // TODO: Might want a copy that takes a ResizeableArray as well
     method WriteRangeArray(start: nat, other: ImmutableArray<T>)
@@ -93,7 +83,14 @@ module {:extern} {:options "/functionSyntax:4"} Arrays {
 
   datatype ArrayCell<T> = Set(value: T) | Unset
 
-  trait {:extern} ImmutableArray<+T> {
+  method {:extern} NewArray<T>(length: nat) returns (ret: Array<T>)
+    ensures ret.Valid()
+    ensures fresh(ret.Repr)
+    ensures ret.Length() == length
+
+  // Separate type in order to have a type with a Valid()
+  // that reads {}.
+  trait {:extern} {:termination false} ImmutableArray<+T> {
 
     ghost const values: seq<T>
 
@@ -135,8 +132,8 @@ module {:extern} {:options "/functionSyntax:4"} Arrays {
       ensures Value() == []
       ensures fresh(Repr)
     {
-      // TODO: Replace with extern to create native array
-      storage := new DafnyArray<T>(length);
+      var storage := NewArray<T>(length);
+      this.storage := storage;
       size := 0;
       new;
       Repr := {this} + storage.Repr;
@@ -188,7 +185,7 @@ module {:extern} {:options "/functionSyntax:4"} Arrays {
       ensures storage.Length() == newCapacity
       ensures Value() == old(Value())
     {
-      var newStorage := new DafnyArray<T>(newCapacity);
+      var newStorage := NewArray<T>(newCapacity);
       var values := storage.Freeze(size);
       newStorage.WriteRangeArray(0, values);
       storage := newStorage;
@@ -230,167 +227,6 @@ module {:extern} {:options "/functionSyntax:4"} Arrays {
       // Explicitly doesn't ensure Valid()!
     {
       ret := storage.Freeze(size);
-    }
-  }
-
-  ///
-  // Feasibility implementation
-  // TODO: Move this to test/ or examples/,
-  // especially since we don't want to compile any seq<T> values
-  ///
-
-  class DafnyArray<T> extends Array<T> {
-    const valuesArray: array<ArrayCell<T>>
-
-    ghost predicate Valid()
-      reads this, Repr
-      ensures Valid() ==> this in Repr
-    {
-      && Repr == {this, valuesArray}
-      && valuesArray[..] == values
-    }
-
-    constructor(length: nat) 
-      ensures Valid()
-      ensures fresh(Repr)
-      ensures values == seq(length, i => Unset)
-    {
-      valuesArray := new ArrayCell<T>[length](i => Unset);
-      new;
-      values := valuesArray[..];
-      Repr := {this, valuesArray};
-    }
-
-    function Length(): nat
-      requires Valid()
-      reads Repr
-      ensures Length() == |values|
-    {
-      valuesArray.Length
-    }
-
-    function Read(i: nat): (ret: T)
-      requires Valid()
-      requires i < Length()
-      requires values[i].Set?
-      reads this, Repr
-      ensures ret == values[i].value
-    {
-      valuesArray[i].value
-    }
-
-    method Write(i: nat, t: T)
-      requires Valid()
-      requires i < Length()
-      modifies Repr
-      ensures Valid()
-      ensures Repr == old(Repr)
-      ensures Length() == old(Length())
-      ensures values == old(values)[..i] + [Set(t)] + old(values)[(i + 1)..]
-      ensures Read(i) == t
-    {
-      valuesArray[i] := Set(t);
-
-      values := valuesArray[..];
-    }
-
-    method WriteRange(start: nat, from: seq<T>)
-      requires Valid()
-      requires start <= Length()
-      requires start + |from| <= Length()
-      modifies Repr
-      ensures Valid()
-      ensures Repr == old(Repr)
-      ensures values == 
-        old(values)[..start] + 
-        seq(|from|, i requires 0 <= i < |from| => Set(from[i])) + 
-        old(values)[(start + |from|)..]
-    {
-      forall i | 0 <= i < |from| {
-        valuesArray[start + i] := Set(from[i]);
-      }
-      values := valuesArray[..];
-    }
-
-    method WriteRangeArray(start: nat, other: ImmutableArray<T>)
-      requires Valid()
-      requires other.Valid()
-      requires start <= Length()
-      requires start + other.Length() <= Length()
-      modifies Repr
-      ensures Valid()
-      ensures Repr == old(Repr)
-      ensures values == 
-        old(values)[..start] + 
-        other.CellValues() +
-        old(values)[(start + other.Length())..]
-    {
-      forall i | 0 <= i < other.Length() {
-        valuesArray[start + i] := Set(other.At(i));
-      }
-      values := valuesArray[..];
-    }
-
-    method Freeze(size: nat) returns (ret: ImmutableArray<T>)
-      requires Valid()
-      requires size <= Length()
-      requires forall i | 0 <= i < size :: values[i].Set?
-      ensures ret.Valid()
-      ensures |ret.values| == size
-      ensures forall i | 0 <= i < size :: ret.values[i] == values[i].value
-    {
-      ret := new DafnyImmutableArray(this, size);
-    }
-  }
-
-  class DafnyImmutableArray<T> extends ImmutableArray<T> {
-
-    const valuesSeq: seq<T>
-
-    ghost predicate Valid() {
-      values == valuesSeq
-    }
-
-    constructor(a: Array<T>, size: nat)
-      requires a.Valid()
-      requires size <= a.Length()
-      requires forall i | 0 <= i < size :: a.values[i].Set?
-      ensures Valid()
-      ensures |values| == size
-      ensures forall i | 0 <= i < size :: values[i] == a.values[i].value
-    {
-      var valuesSeq := ValuesFromArray(a, size);
-      this.values := valuesSeq;
-      this.valuesSeq := valuesSeq;
-    }
-
-    static function ValuesFromArray(a: Array<T>, size: nat): (ret: seq<T>)
-      requires a.Valid()
-      requires size <= a.Length()
-      requires forall i | 0 <= i < size :: a.values[i].Set?
-      reads a, a.Repr
-      ensures |ret| == size
-      ensures forall i | 0 <= i < size :: ret[i] == a.values[i].value
-    {
-      if size == 0 then
-        []
-      else
-        ValuesFromArray(a, size - 1) + [a.Read(size - 1)]
-    }
-
-    function Length(): nat 
-      requires Valid()
-      ensures Length() == |values|
-    {
-      |valuesSeq|
-    }
-
-    function At(index: nat): T
-      requires Valid()
-      requires index < |values|
-      ensures At(index) == values[index]
-    {
-      valuesSeq[index]
     }
   }
 }
