Source/DafnyRuntime/DafnyRuntimeDafny/test/DafnyArray.dfy
@@ -1,0 +1,149 @@
+
+include "../src/array.dfy"
+
+
+module {:options "/functionSyntax:4"} DafnyArrays {
+  import opened Arrays
+
+  ///
+  // Feasibility implementation
+  // TODO: Move this to test/ or examples/,
+  // especially since we don't want to compile any seq<T> values
+  ///
+  class DafnyArray<T> extends Array<T> {
+    const valuesArray: array<ArrayCell<T>>
+
+    ghost predicate Valid()
+      reads this, Repr
+      ensures Valid() ==> this in Repr
+    {
+      && Repr == {this, valuesArray}
+      && valuesArray[..] == values
+    }
+
+    constructor(length: nat)
+      ensures Valid()
+      ensures fresh(Repr)
+      ensures values == seq(length, i => Unset)
+    {
+      valuesArray := new ArrayCell<T>[length](i => Unset);
+      new;
+      values := valuesArray[..];
+      Repr := {this, valuesArray};
+    }
+
+    function Length(): nat
+      requires Valid()
+      reads Repr
+      ensures Length() == |values|
+    {
+      valuesArray.Length
+    }
+
+    function Read(i: nat): (ret: T)
+      requires Valid()
+      requires i < Length()
+      requires values[i].Set?
+      reads this, Repr
+      ensures ret == values[i].value
+    {
+      valuesArray[i].value
+    }
+
+    method Write(i: nat, t: T)
+      requires Valid()
+      requires i < Length()
+      modifies Repr
+      ensures Valid()
+      ensures Repr == old(Repr)
+      ensures Length() == old(Length())
+      ensures values == old(values)[..i] + [Set(t)] + old(values)[(i + 1)..]
+      ensures Read(i) == t
+    {
+      valuesArray[i] := Set(t);
+
+      values := valuesArray[..];
+    }
+
+    method WriteRangeArray(start: nat, other: ImmutableArray<T>)
+      requires Valid()
+      requires other.Valid()
+      requires start <= Length()
+      requires start + other.Length() <= Length()
+      modifies Repr
+      ensures Valid()
+      ensures Repr == old(Repr)
+      ensures values == 
+        old(values)[..start] + 
+        other.CellValues() +
+        old(values)[(start + other.Length())..]
+    {
+      forall i | 0 <= i < other.Length() {
+        valuesArray[start + i] := Set(other.At(i));
+      }
+      values := valuesArray[..];
+    }
+
+    method Freeze(size: nat) returns (ret: ImmutableArray<T>)
+      requires Valid()
+      requires size <= Length()
+      requires forall i | 0 <= i < size :: values[i].Set?
+      ensures ret.Valid()
+      ensures |ret.values| == size
+      ensures forall i | 0 <= i < size :: ret.values[i] == values[i].value
+    {
+      ret := new DafnyImmutableArray(this, size);
+    }
+  }
+
+  class DafnyImmutableArray<T> extends ImmutableArray<T> {
+
+    const valuesSeq: seq<T>
+
+    ghost predicate Valid() {
+      values == valuesSeq
+    }
+
+    constructor(a: Array<T>, size: nat)
+      requires a.Valid()
+      requires size <= a.Length()
+      requires forall i | 0 <= i < size :: a.values[i].Set?
+      ensures Valid()
+      ensures |values| == size
+      ensures forall i | 0 <= i < size :: values[i] == a.values[i].value
+    {
+      var valuesSeq := ValuesFromArray(a, size);
+      this.values := valuesSeq;
+      this.valuesSeq := valuesSeq;
+    }
+
+    static function ValuesFromArray(a: Array<T>, size: nat): (ret: seq<T>)
+      requires a.Valid()
+      requires size <= a.Length()
+      requires forall i | 0 <= i < size :: a.values[i].Set?
+      reads a, a.Repr
+      ensures |ret| == size
+      ensures forall i | 0 <= i < size :: ret[i] == a.values[i].value
+    {
+      if size == 0 then
+        []
+      else
+        ValuesFromArray(a, size - 1) + [a.Read(size - 1)]
+    }
+
+    function Length(): nat 
+      requires Valid()
+      ensures Length() == |values|
+    {
+      |valuesSeq|
+    }
+
+    function At(index: nat): T
+      requires Valid()
+      requires index < |values|
+      ensures At(index) == values[index]
+    {
+      valuesSeq[index]
+    }
+  }
+}
